Core.v
@@ -3,3 +3,4 @@ From Elo Require Export Array.
 From Elo Require Export Map.
 From Elo Require Export Sem.
 From Elo Require Export SemExt.
+From Elo Require Export Values.
