Values.v
@@ -1,0 +1,16 @@
+From Elo Require Import Sem.
+From Elo Require Import SemExt.
+
+Lemma value_init_term : forall t1 t2 ad t,
+  t1 --[e_init ad t]--> t2 ->
+  value t.
+Proof.
+  intros. ind_tstep; eauto.
+Qed.
+
+Lemma value_write_term : forall t1 t2 ad t,
+  t1 --[e_write ad t]--> t2 ->
+  value t.
+Proof.
+  intros. ind_tstep; eauto.
+Qed.
